updates

intermediate/Veritas.Intermediate.Store.fsti
@@ -4,6 +4,7 @@ open Veritas.BinTree
 open Veritas.Key
 open Veritas.Record
 open Veritas.SeqAux
+open Veritas.Intermediate.VerifierConfig
 
 module Spec = Veritas.Verifier
 module FE = FStar.FunctionalExtensionality
@@ -12,60 +13,60 @@ module FE = FStar.FunctionalExtensionality
 
 let add_method = Veritas.Verifier.add_method
 
+(* an index in store *)
+let slot_id (vcfg:verifier_config) = i:nat{i < store_size vcfg}
+
 (* 
  * vstore_entry - reflect a Spec.vstore_entry with two additional fields tracking 
  * whether a left/right descendant was added using merkle using this slot as "proof"
  *)
-type vstore_entry = 
+type vstore_entry (vcfg:verifier_config) = 
   | VStoreE: k:key -> 
              v:value_type_of k -> 
              am:add_method -> 
-             l_in_store : option nat{is_merkle_key k \/ None = l_in_store} -> 
-             r_in_store : option nat{is_merkle_key k \/ None = r_in_store} -> 
-             vstore_entry
+             l_in_store : option (slot_id vcfg){is_merkle_key k \/ None = l_in_store} -> 
+             r_in_store : option (slot_id vcfg){is_merkle_key k \/ None = r_in_store} -> 
+             vstore_entry vcfg
 
 (* vstore_raw: the raw version of the vstore; the actual vstore 
  * is the raw version with some invariants *)
-type vstore_raw = Seq.seq (option vstore_entry) 
+let vstore_raw vcfg = st:Seq.seq (option (vstore_entry vcfg)){Seq.length st = store_size vcfg}
 
-(* an index in store *)
-let slot_id (st:vstore_raw) = seq_index st
-
-let get_slot (st:vstore_raw) (s: slot_id st)
-  : option vstore_entry
+let get_slot #vcfg (st:vstore_raw vcfg) (s: slot_id vcfg)
+  : option (vstore_entry vcfg)
   = Seq.index st s
 
 (* return true if s is a valid slot that is occupied *)
-let inuse_slot (st:vstore_raw) (s:slot_id st) : bool
+let inuse_slot #vcfg (st:vstore_raw vcfg) (s:slot_id vcfg) : bool
   = Some? (get_slot st s)
 
 (* dep type of all slots in use *)
-let inuse_slot_id (st: vstore_raw) = s:slot_id st{inuse_slot st s}
+let inuse_slot_id #vcfg (st: vstore_raw vcfg) = s:slot_id vcfg{inuse_slot st s}
 
-let get_inuse_slot (st:vstore_raw) (s:inuse_slot_id st) =
+let get_inuse_slot #vcfg (st:vstore_raw vcfg) (s:inuse_slot_id st) =
   Some?.v (get_slot st s)
 
 (* is this an empty slot *)
-let empty_slot (st:vstore_raw) (s:slot_id st): bool 
+let empty_slot #vcfg (st:vstore_raw vcfg) (s:slot_id vcfg): bool 
   = None = get_slot st s
 
-let empty_slot_id (st: vstore_raw) = s:slot_id st{empty_slot st s}
+let empty_slot_id #vcfg (st: vstore_raw vcfg) = s:slot_id vcfg{empty_slot st s}
 
 (* key stored at an occupied slot *)
-let stored_key (st:vstore_raw) (s:inuse_slot_id st) : key
+let stored_key #vcfg (st:vstore_raw vcfg) (s:inuse_slot_id st) : key
   = VStoreE?.k (Some?.v (get_slot st s))
 
 (* is this a slot containing a merkle key *)
-let merkle_slot_id (st:vstore_raw)
+let merkle_slot_id #vcfg (st:vstore_raw vcfg)
   = s:inuse_slot_id st{is_merkle_key (stored_key st s)}
 
-let data_slot_id (st:vstore_raw)
+let data_slot_id #vcfg (st:vstore_raw vcfg)
   = s:inuse_slot_id st{is_data_key (stored_key st s)}
 
-let stored_value (st:vstore_raw) (s:inuse_slot_id st) : value
+let stored_value #vcfg (st:vstore_raw vcfg) (s:inuse_slot_id st) : value
   = VStoreE?.v (Some?.v (get_slot st s))
 
-let add_method_of (st:vstore_raw) (s:inuse_slot_id st) : add_method
+let add_method_of #vcfg (st:vstore_raw vcfg) (s:inuse_slot_id st) : add_method
   = VStoreE?.am (Some?.v (get_slot st s))
 
 (* TODO: Move to a better place ?*)
@@ -79,101 +80,99 @@ let mv_pointed_key (mv:merkle_value) (d:bin_tree_dir{mv_points_to_some mv d}) : 
   = Desc?.k (desc_hash_dir mv d)
 
 (* was a descendant added with MAdd along direction d *)
-let desc_in_store (st:vstore_raw) (s:inuse_slot_id st) (d:bin_tree_dir) : bool
+let desc_in_store #vcfg (st:vstore_raw vcfg) (s:inuse_slot_id st) (d:bin_tree_dir) : bool
   = match d with
     | Left -> Some? (VStoreE?.l_in_store (Some?.v (get_slot st s)))
     | Right -> Some? (VStoreE?.r_in_store (Some?.v (get_slot st s)))
 
 (* if a descendant was added with MAdd, the slot where the descendant was added *)
-let desc_slot_raw (st:vstore_raw) (s:inuse_slot_id st) (d:bin_tree_dir{desc_in_store st s d}): nat
+let desc_slot #vcfg (st:vstore_raw vcfg) (s:inuse_slot_id st) (d:bin_tree_dir{desc_in_store st s d}): slot_id vcfg
   = match d with
     | Left -> Some?.v (VStoreE?.l_in_store (Some?.v (get_slot st s)))
     | Right -> Some?.v (VStoreE?.r_in_store (Some?.v (get_slot st s)))
 
-(* invariant connecting the value stored in a slot and the desc info *)
-let desc_in_store_inv_merkle (st:vstore_raw) (s:merkle_slot_id st) (d:bin_tree_dir) = 
+(* invariant connecting the value stored in a merkle slot and the desc info *)
+let desc_in_store_inv_merkle #vcfg (st:vstore_raw vcfg) (s:merkle_slot_id st) (d:bin_tree_dir) = 
   let v = to_merkle_value (stored_value st s) in
   mv_points_to_none v d /\ not (desc_in_store st s d) \/
   mv_points_to_some v d /\ (desc_in_store st s d ==> 
-                            (let ds = desc_slot_raw st s d in
-                             ds < Seq.length st /\               // valid slot_id                 
-                             (let dk = mv_pointed_key v d in
+                            (let ds = desc_slot st s d in
+                             let dk = mv_pointed_key v d in
                               inuse_slot st ds /\                // slot_id in use                              
                               stored_key st ds = dk /\           // stored key is the key in my value
-                              add_method_of st ds = Spec.MAdd))) // Merkle add
+                              add_method_of st ds = Spec.MAdd))  // Merkle add
 
-let desc_in_store_inv_data (st:vstore_raw) (s:data_slot_id st) = 
+(* invariant connecting value stored in a data slot and desc info *)
+let desc_in_store_inv_data #vcfg (st:vstore_raw vcfg) (s:data_slot_id st) = 
   not (desc_in_store st s Left) && 
   not (desc_in_store st s Right)
 
-let store_inv_slot (st:vstore_raw) (s:slot_id st) = 
+(* general invariant for all slots: a slot is empty or satisfies the invariant for merkle/data *)
+let store_inv_slot #vcfg (st:vstore_raw vcfg) (s:slot_id vcfg) = 
   empty_slot st s \/
   (is_data_key (stored_key st s) /\ desc_in_store_inv_data st s) \/
   (is_merkle_key (stored_key st s) /\ 
    desc_in_store_inv_merkle st s Left /\ 
    desc_in_store_inv_merkle st s Right)
 
-let store_inv_local (st:vstore_raw) = 
-  forall (s:slot_id st). store_inv_slot st s
+let store_inv_local #vcfg (st:vstore_raw vcfg) = 
+  forall (s:slot_id vcfg). store_inv_slot st s
 
-let vstore = st:vstore_raw{store_inv_local st}
+(* vstore is a raw store that satisfies the local invariant *)
+let vstore vcfg = st:vstore_raw vcfg{store_inv_local st}
 
-let empty_store (n:nat) :vstore = Seq.create n None
+let empty_store vcfg:vstore vcfg = Seq.create (store_size vcfg) None
   
-let has_key (k:key) (e:option vstore_entry) : bool
+let has_key #vcfg (k:key) (e:option (vstore_entry vcfg)) : bool
   = match e with
     | Some (VStoreE k' _ _ _ _) -> k = k'
     | None -> false
-
-(* desc slot verified version that returns a slot id *)
-let desc_slot (st:vstore) 
-              (s:merkle_slot_id st) 
-              (d:bin_tree_dir{desc_in_store st s d}): slot_id st = 
-  desc_slot_raw st s d
 
 (** vstore update methods **)
 
 (* relationship between two stores st and st' that states that 
  * they are of the same size and differ in only one slot *)
-let idx_store_update_rel (st st': vstore) (s:slot_id st) 
-  = Seq.length st = Seq.length st' /\
-    (forall (s':slot_id st). (s' <> s ==> get_slot st s' == get_slot st' s'))
+let idx_store_update_rel #vcfg (st st': vstore vcfg) (s:slot_id vcfg) 
+  = (forall (s':slot_id vcfg). (s' <> s ==> get_slot st s' == get_slot st' s'))
 
 (* add a new entry (k,v) to the store at en empty slot s; *)
 val add_to_store 
-      (st:vstore) 
+      (#vcfg:verifier_config)
+      (st:vstore vcfg) 
       (s:empty_slot_id st)
       (k:key) 
       (v:value_type_of k) 
       (am:add_method)
-  : Tot (st':vstore {idx_store_update_rel st st' s /\
-                     inuse_slot st' s /\
-                     get_inuse_slot st' s = VStoreE k v am None None})
+  : Tot (st':vstore vcfg {idx_store_update_rel st st' s /\
+                          inuse_slot st' s /\
+                          get_inuse_slot st' s = VStoreE k v am None None})
 
 (* add a new entry with merkle and a descendant *)
 (* TODO: Add when this is used *)
 val add_to_store_with_desc
-      (st:vstore)
+      (#vcfg:_)
+      (st:vstore vcfg)
       (s:empty_slot_id st)
       (k:merkle_key)
       (v:merkle_value)
       (d:bin_tree_dir{mv_points_to_some v d})
       (s':merkle_slot_id st{mv_pointed_key v d = stored_key st s'})
-  : Tot (st':vstore {idx_store_update_rel st st' s /\
-                     inuse_slot st' s /\
-                     stored_key st' s = k /\
-                     stored_value st' s = (MVal v) /\
-                     add_method_of st' s = Spec.MAdd /\
-                     desc_in_store st' s d /\
-                     desc_slot st' s d = s' /\
-                     not (desc_in_store st' s d)})
+  : Tot (st':vstore vcfg {idx_store_update_rel st st' s /\
+                          inuse_slot st' s /\
+                          stored_key st' s = k /\
+                          stored_value st' s = (MVal v) /\
+                          add_method_of st' s = Spec.MAdd /\
+                          desc_in_store st' s d /\
+                          desc_slot st' s d = s' /\
+                          not (desc_in_store st' s d)})
                      
 (* update the data value of a data key *)
 val update_data_value 
-  (st:vstore)
+  (#vcfg:_)
+  (st:vstore vcfg)
   (s:data_slot_id st)
   (v:data_value)
-  : Tot (st':vstore {
+  : Tot (st':vstore vcfg {
         let VStoreE k _ am _ _ = get_inuse_slot st s in
         (idx_store_update_rel st st' s /\
          inuse_slot st' s /\
@@ -181,13 +180,30 @@ val update_data_value
 
 (* reset a descendant of a merkle slot *)
 val reset_desc_slot
-  (st:vstore)
+  (#vcfg:_)
+  (st:vstore vcfg)
   (s:merkle_slot_id st)
   (d:bin_tree_dir{desc_in_store st s d})
-  : Tot (st': vstore {idx_store_update_rel st st' s /\
-                      inuse_slot st' s /\ 
-                      stored_key st' s = stored_key st s /\
-                      not (desc_in_store st s d)})
+  : Tot (st': vstore vcfg {idx_store_update_rel st st' s /\
+                           inuse_slot st' s /\ 
+                           stored_key st' s = stored_key st s /\
+                           not (desc_in_store st s d)})
+
+(* when the current desc slot along a direction is empty, add a desc slot along that direction *)
+val add_desc_slot
+  (#vcfg:_)
+  (st:vstore vcfg)
+  (s:merkle_slot_id st)
+  (d:bin_tree_dir{not (desc_in_store st s d)})
+  (s':inuse_slot_id st{let v = to_merkle_value (stored_value st s) in
+                       mv_points_to_some v d /\
+                       mv_pointed_key v d = stored_key st s'})
+  : Tot (st':vstore vcfg {idx_store_update_rel st st' s /\
+                          inuse_slot st' s /\
+                          (let VStoreE k v am ld rd = get_inuse_slot st s in
+                           match d with
+                           | Left -> get_inuse_slot st' s = VStoreE k v am (Some s') rd 
+                           | Right -> get_inuse_slot st' s = VStoreE k v am ld (Some s'))})
 
 (* two values point to the same key along some dir (or don't point to any) *)
 let points_to_same (v1 v2: merkle_value) (d:bin_tree_dir) = 
@@ -195,41 +211,71 @@ let points_to_same (v1 v2: merkle_value) (d:bin_tree_dir) =
   mv_points_to_some v1 d && mv_points_to_some v2 d && 
   mv_pointed_key v1 d = mv_pointed_key v2 d
 
-(* update a merkle value with a new value that points to the same keys *)
+(* change the merkle value along a given direction *)
 val update_merkle_value
-  (st:vstore)
+  (#vcfg:_)
+  (st:vstore vcfg)
   (s:merkle_slot_id st)
-  (v:merkle_value {let vold = to_merkle_value (stored_value st s) in
-                   points_to_same v vold Left &&
-                   points_to_same v vold Right})
-  : Tot (st': vstore {idx_store_update_rel st st' s /\
-                      inuse_slot st' s /\
-                      (let VStoreE k _ am ld rd = get_inuse_slot st s in
-                       get_inuse_slot st' s = VStoreE k (MVal v) am ld rd)})
+  (d: bin_tree_dir)
+  (k: key) (h:hash_value) (b:bool)
+  (s':inuse_slot_id st{k = stored_key st s'})  
+  : Tot (st': vstore vcfg {idx_store_update_rel st st' s /\
+                           inuse_slot st' s /\
+                           (let VStoreE k1 v1 am1 ld1 rd1 = get_inuse_slot st s in
+                            let VStoreE k2 v2 am2 ld2 rd2 = get_inuse_slot st' s in
+                            k1 = k2 /\
+                            am1 = am2 /\
+                            to_merkle_value v2 = Spec.update_merkle_value (to_merkle_value v1) d k h b /\
+                            ld2 = (if d = Left then Some s' else ld1) /\
+                            rd2 = (if d = Right then Some s' else rd2))})
 
+val update_empty_merkle_value 
+  (#vcfg:_)
+  (st:vstore vcfg)
+  (s:merkle_slot_id st)
+  (d:bin_tree_dir)
+  (s':inuse_slot_id st)
+  (v:merkle_value {let vold = to_merkle_value (stored_value st s) in
+                   let do = other_dir d in
+                   let k' = stored_key st s' in
+                   desc_hash_dir v do = desc_hash_dir vold do && // v and vold are same in dir (1 - d)
+                   mv_points_to_none vold d &&                   // vold points to none in direction d
+                   mv_points_to_some v d &&                      // v points to key k' in slot s'
+                   mv_pointed_key v d = k'})
+  : Tot (st': vstore vcfg {let do = other_dir d in
+                           idx_store_update_rel st st' s /\
+                           inuse_slot st' s /\
+                           desc_in_store st' s d /\               // s points to s' in direction d 
+                           desc_slot st' s d = s' /\ 
+                           desc_in_store st' s do = desc_in_store st s do /\
+                           desc_in_store st' s do ==> desc_slot st' s do = desc_slot st s do /\
+                           stored_key st' s = stored_key st s /\
+                           stored_value st' s = (MVal v) /\
+                           add_method_of st' s = add_method_of st s})
+                                                     
 (* remove an entry from a slot; reset slot to unused *)
-val evict_from_store (st:vstore) (s:inuse_slot_id st)
-  : Tot (st':vstore {idx_store_update_rel st st' s /\
-                     empty_slot st' s})
+val evict_from_store (#vcfg:_) (st:vstore vcfg) (s:inuse_slot_id st)
+  : Tot (st':vstore vcfg {idx_store_update_rel st st' s /\
+                          empty_slot st' s})
 
 (* if the store contains key k, return some entry in the store, otherwise return None *)
-let lookup_key (st:vstore) (k:key) 
-  : option vstore_entry
+let lookup_key (#vcfg:_) (st:vstore vcfg) (k:key) 
+  : option (vstore_entry vcfg)
   = let s' = filter (has_key k) st in
     if Seq.length s' = 0 then None
     else Seq.index s' 0 
 
-let store_contains_key (st:vstore) (k:key) : bool
+let store_contains_key #vcfg (st:vstore vcfg) (k:key) : bool
   = Some? (lookup_key st k)
 
-val lemma_store_contains_key (st:vstore) (k:key)
+val lemma_store_contains_key (#vcfg:_) (st:vstore vcfg) (k:key)
   : Lemma (requires (exists s. stored_key st s = k))
           (ensures (store_contains_key st k))
           [SMTPat (store_contains_key st k)]
 
-val stored_value_by_key (st:vstore) (k:key{store_contains_key st k}) : value_type_of k
+val stored_value_by_key  (#vcfg:_) (st:vstore vcfg) (k:key{store_contains_key st k}) : value_type_of k
 
-val add_method_of_by_key (st:vstore) (k:key{store_contains_key st k}) : add_method
+val add_method_of_by_key (#vcfg:_) (st:vstore vcfg) (k:key{store_contains_key st k}) : add_method
 
 (*** Store Invariants ***)
 
@@ -240,14 +286,14 @@ val add_method_of_by_key (st:vstore) (k:key{store_contains_key st k}) : add_meth
 *)
 
 (* No duplicate keys in the store *)
-let is_map (st:vstore) =
+let is_map (#vcfg:_) (st:vstore vcfg) =
   forall (s:inuse_slot_id st) 
     (s':inuse_slot_id st{s' <> s}). 
         // TODO: this pattern is pretty general -- it may lead to proof performance issues
         {:pattern (Seq.index st s); (Seq.index st s')} 
     stored_key st s <> stored_key st s'
 
-let elim_is_map (st:vstore) 
+let elim_is_map (#vcfg:_) (st:vstore vcfg) 
                 (s:inuse_slot_id st)
                 (s':inuse_slot_id st{s' <> s})
   : Lemma (requires is_map st)
@@ -255,11 +301,12 @@ let elim_is_map (st:vstore)
   = ()
 
 (* a store that is a map *)
-let ismap_vstore = st:vstore{is_map st}
+let ismap_vstore vcfg = st:vstore vcfg{is_map st}
 
 (* updating a data value preserves is_map *)
 val lemma_update_data_value_preserves_is_map
-      (st:ismap_vstore)
+      (#vcfg:_)
+      (st:ismap_vstore vcfg)
       (s:data_slot_id st)
       (v:data_value)
   : Lemma (ensures (is_map (update_data_value st s v)))
@@ -267,24 +314,27 @@ val lemma_update_data_value_preserves_is_map
 
 (* reset desc slot preserves is_map *)
 val lemma_reset_desc_slot_preserves_is_map
-      (st:ismap_vstore)
+      (#vcfg:_)
+      (st:ismap_vstore vcfg)
       (s:merkle_slot_id st)
       (d:bin_tree_dir{desc_in_store st s d})
   : Lemma (ensures (is_map (reset_desc_slot st s d)))
           [SMTPat (is_map (reset_desc_slot st s d))]
 
 val lemma_update_merkle_value
-      (st:ismap_vstore)
+      (#vcfg:_)
+      (st:ismap_vstore vcfg)
       (s:merkle_slot_id st)
-      (v:merkle_value {let vold = to_merkle_value (stored_value st s) in
-                       points_to_same v vold Left &&
-                       points_to_same v vold Right})
-  : Lemma (ensures (is_map (update_merkle_value st s v)))
-          [SMTPat (is_map (update_merkle_value st s v))]
+      (d:bin_tree_dir)
+      (k: key) (h:hash_value) (b:bool)
+      (s':inuse_slot_id st{k = stored_key st s'})
+  : Lemma (ensures (is_map (update_merkle_value st s d k h b s')))
+          [SMTPat (is_map (update_merkle_value st s d k h b s'))]
 
 (* is_map is preserved when adding a new key *)
 val lemma_add_to_store_is_map1
-      (st:ismap_vstore) 
+      (#vcfg:_)
+      (st:ismap_vstore vcfg) 
       (s:empty_slot_id st) 
       (k:key{not (store_contains_key st k)}) 
       (v:value_type_of k) 
@@ -294,7 +344,8 @@ val lemma_add_to_store_is_map1
 
 (* is_map is violated when adding a duplicate key *)
 val lemma_add_to_store_is_map2
-      (st:vstore) 
+      (#vcfg:_)
+      (st:vstore vcfg) 
       (s:empty_slot_id st) 
       (k:key{store_contains_key st k}) 
       (v:value_type_of k) 
@@ -302,14 +353,14 @@ val lemma_add_to_store_is_map2
   : Lemma (ensures (~ (is_map (add_to_store st s k v am))))
           [SMTPat (is_map (add_to_store st s k v am))]
 
-val lemma_evict_from_store_preserves_is_map (st:ismap_vstore) (s:inuse_slot_id st)
+val lemma_evict_from_store_preserves_is_map (#vcfg:_) (st:ismap_vstore vcfg) (s:inuse_slot_id st)
   : Lemma (ensures (is_map (evict_from_store st s)))
           [SMTPat (is_map (evict_from_store st s))]
 
 (*** Relation w/ Spec-level Stores ***)
 
 (* slot_id s is equivalent to key k *)
-let slot_key_equiv (st:vstore) (s:slot_id st) (k:key) : bool =
+let slot_key_equiv #vcfg (st:vstore vcfg) (s:slot_id vcfg) (k:key) : bool =
   inuse_slot st s && stored_key st s = k 
 
 (*
@@ -326,14 +377,13 @@ val lemma_slot_key_equiv_update_value
 *)
 
 (* convert a slot-indexed store to a key-indexed store *)
-val as_map (st:ismap_vstore) : Spec.vstore
+val as_map (#vcfg:_) (st:ismap_vstore vcfg) : Spec.vstore
 
-val lemma_as_map_empty (n:nat) 
-  : Lemma (ensures (let st = empty_store n in
+val lemma_as_map_empty (vcfg:_)
+  : Lemma (ensures (let st = empty_store vcfg in
                      forall (k:key). as_map st k = None))
-          (decreases n)
 
-val lemma_as_map_slot_key_equiv (st:ismap_vstore) (s:slot_id st) (k:key)
+val lemma_as_map_slot_key_equiv (#vcfg:_) (st:ismap_vstore vcfg) (s:slot_id vcfg) (k:key)
   : Lemma (requires (slot_key_equiv st s k)) 
           (ensures (Spec.store_contains (as_map st) k /\
                     stored_value st s = Spec.stored_value (as_map st) k /\
@@ -341,20 +391,20 @@ val lemma_as_map_slot_key_equiv (st:ismap_vstore) (s:slot_id st) (k:key)
           [SMTPat (slot_key_equiv st s k)]
 
 (* Relation between stores *)
-let store_rel (st:vstore) (st':Spec.vstore) : Type = 
+let store_rel (#vcfg:_) (st:vstore vcfg) (st':Spec.vstore) : Type = 
   is_map st /\ FE.feq st' (as_map st)
 
-val lemma_store_rel_contains_key (st:vstore) (st':Spec.vstore) (k:key)
+val lemma_store_rel_contains_key (#vcfg:_) (st:vstore vcfg) (st':Spec.vstore) (k:key)
   : Lemma (requires (store_rel st st'))
           (ensures (store_contains_key st k = Spec.store_contains st' k))
           [SMTPat (store_contains_key st k); SMTPat (Spec.store_contains st' k)]
 
-val lemma_store_rel_stored_value (st:vstore) (st':Spec.vstore) (k:key)
+val lemma_store_rel_stored_value (#vcfg:_) (st:vstore vcfg) (st':Spec.vstore) (k:key)
   : Lemma (requires (store_rel st st' /\ store_contains_key st k))
           (ensures (stored_value_by_key st k = Spec.stored_value st' k))
           [SMTPat (stored_value_by_key st k); SMTPat (Spec.stored_value st' k)]
 
-val lemma_store_rel_add_method_of (st:vstore) (st':Spec.vstore) (k:key)
+val lemma_store_rel_add_method_of (#vcfg:_) (st:vstore vcfg) (st':Spec.vstore) (k:key)
   : Lemma (requires (store_rel st st' /\ store_contains_key st k))
           (ensures (add_method_of_by_key st k = Spec.add_method_of st' k))
           [SMTPat (add_method_of_by_key st k); SMTPat (Spec.add_method_of st' k)]
@@ -372,7 +422,8 @@ val lemma_store_rel_update_in_store (st:vstore) (st':Spec.vstore) (s:slot_id) (d
 *)
 
 val lemma_store_rel_add_to_store 
-      (st:vstore) 
+      (#vcfg:_)
+      (st:vstore vcfg) 
       (st':Spec.vstore) 
       (s:empty_slot_id st) 
       (k:key) 
@@ -382,7 +433,7 @@ val lemma_store_rel_add_to_store
           (ensures (store_rel (add_to_store st s k v am) (Spec.add_to_store st' k v am)))
           [SMTPat (add_to_store st s k v am); SMTPat (Spec.add_to_store st' k v am)]
 
-val lemma_store_rel_evict_from_store (st:vstore) (st':Spec.vstore) (s:slot_id st) (k:key)
+val lemma_store_rel_evict_from_store (#vcfg:_) (st:vstore vcfg) (st':Spec.vstore) (s:slot_id vcfg) (k:key)
   : Lemma (requires (store_rel st st' /\ slot_key_equiv st s k))
           (ensures (store_rel (evict_from_store st s) (Spec.evict_from_store st' k)))
           [SMTPat (evict_from_store st s); SMTPat (Spec.evict_from_store st' k)]
