intermediate/Veritas.Intermediate.VerifierConfig.fsti
@@ -1,0 +1,7 @@
+module Veritas.Intermediate.VerifierConfig
+
+type verifier_config = 
+  | VConfig: store_size: nat -> nthreads: nat -> verifier_config
+
+let store_size (vc: verifier_config): nat = 
+  VConfig?.store_size vc
